endian conversion added to C code generation

src/Verse/Arch/C.v
@@ -17,6 +17,7 @@ Require Import Ensembles.
 Require Import Program.Basics.
 Require Vector.
 Import Vector.VectorNotations.
+Require Import Arith.
 Set Implicit Arguments.
 
 Module CP.
@@ -36,7 +37,7 @@ Module CP.
   Definition plusplus d            := text "++" <> d.
   Definition minusminus d          := text "--" <> d.
 
-  Definition comment s   := between ("/*    ") ("    */") (text s).
+  Definition comment s   := PrettyPrint.between ("/*    ") ("    */") (text s).
   Definition blockPtrVariableName := "blockPtr".
 
 End CP.
@@ -80,8 +81,78 @@ Instance cMachineVar : forall k (ty : type k), PrettyPrint (cvar ty)
                        end
      }.
 
+Section PrintingInstruction.
 
+  Definition wordSize (ty : type direct) := match ty with
+                                            | word w => decimal (2 ^ (w + 3))%nat
+                                            | _      => text "Unsupported"
+                                            end.
 
+  Definition toLE ty v := text ("verse_to_le") <> wordSize ty <> paren v.
+  Definition toBE ty v := text ("verse_to_be") <> wordSize ty <> paren v.
+  Definition fromLE ty v := text ("verse_from_le") <> wordSize ty <> paren v.
+  Definition fromBE ty v := text ("verse_from_be") <> wordSize ty <> paren v.
+
+  Definition rval {k} {ty : type k} (a : arg cvar _ ty) :=
+    match a with
+    | @Language.index _ _ littleE ty _ _ => fromLE ty (doc a)
+    | @Language.index _ _ bigE ty _ _    => fromBE ty (doc a)
+    | _                                  => doc a
+    end.
+
+  Definition CAssign {a : arity} (o : op a) {k} {ty : type k} (a : arg cvar _ ty) (y z : Doc)  :=
+    match a with
+    | @Language.index _ _ littleE ty _ _ => doc a <_> EQUALS <_> toLE ty (y <_> opDoc o <_> z)
+    | @Language.index _ _ bigE ty _ _ => doc a <_> EQUALS <_> toBE ty (y <_> opDoc o <_> z)
+    | _                                  => doc a <_> EQUALS <_> y <_> opDoc o <_> z
+    end.
+
+  Definition CRot (ty : type direct) (o : op unary) (a : arg cvar _ ty) (y : Doc)  :=
+    let rvl := match o with
+               | rotL n => text "rotL" <> wordSize ty <> paren (commaSep [y ; decimal n])
+               | rotR n => text "rotR" <> wordSize ty <> paren (commaSep [y ; decimal n])
+               | _      => text "BadOp"
+               end
+    in
+    match a with
+    | @Language.index _ _ littleE ty _ _ => doc a <_> EQUALS <_> toLE ty rvl
+    | @Language.index _ _ bigE ty _ _    => doc a <_> EQUALS <_> toBE ty rvl
+    | _                                  => doc a <_> EQUALS <_> rvl
+    end.
+
+  Definition CUpdate {a : arity}(o : op a) {k} {ty : type k} (a : arg cvar _ ty) (y : Doc) :=
+    match a with
+    | @Language.index _ _ littleE ty _ _ => CAssign o a (rval a) y
+    | @Language.index _ _ bigE ty _ _    => CAssign o a (rval a) y
+    | _                                  => doc a <_> opDoc o <> EQUALS <_> y
+    end.
+
+  Global Instance assignment_C_print : PrettyPrint (assignment cvar) | 0
+    := { doc := fun assgn =>  match assgn with
+                              | assign3 o x y z => CAssign o x (rval y) (rval z)
+                              | update2 o x y   => CUpdate o x (rval y)
+                              | @assign2 _ ty u x y   =>
+                                match u with
+                                | bitComp  | nop | mov => CAssign u x empty (rval y)
+                                | shiftL n | shiftR n  => CAssign u x (rval y) (decimal n)
+                                | rotL n   | rotR n    => CRot u x (rval y)
+                                end
+                              | @update1 _ ty u x      =>
+                                match u with
+                                | bitComp  | nop | mov => CAssign u x empty (rval x)
+                                | shiftL n | shiftR n  => CUpdate u x (decimal n)
+                                | rotL n   | rotR n    => CRot u x (rval x)
+                                end
+                              end
+       }.
+
+  Global Instance instruction_C_print : PrettyPrint (instruction cvar) | 0
+    := { doc := fun i => match i with
+                         | assign a => doc a
+                         end
+       }.
+
+End PrintingInstruction.
 
 
 Module C <: ARCH.
@@ -96,15 +167,15 @@ Module C <: ARCH.
 
   Definition machineVar := cvar.
 
-  Definition HostEndian := bigE.
+  Definition HostEndian := hostE.
   
   Definition Word := Word64.
 
   Definition embedRegister := inRegister.
 
-  Definition supportedInst := Language.supportedInst machineVar littleE.
+  Definition supportedInst := Language.supportedInst machineVar hostE.
 
-  Definition instCheck := Language.instCheck machineVar littleE.
+  Definition instCheck := Language.instCheck machineVar hostE.
 
   Inductive typesSupported : forall k, Ensemble (type k) :=
   | uint8           : typesSupported Word8
@@ -199,7 +270,7 @@ Module CCodeGen <: CODEGEN C.
 
   Import C.
 
-  Definition emit (i : instruction (machineVar)) : Doc + { not (supportedInst i) } :=
+  Definition emit (i : instruction machineVar) : Doc + { not (supportedInst i) } :=
     _ <- when instCheck i; {- doc i <> text ";" -}.
 
   Definition sequenceInstructions ds := line <> vcat ds.
